{-# OPTIONS --without-K --safe #-}

open import Definition.Typed.EqualityRelation

module Definition.LogicalRelation.Properties.Neutral {{eqrel : EqRelSet}} where
open EqRelSet {{...}}

open import Definition.Untyped hiding (_∷_)
open import Definition.Untyped.Properties
open import Definition.Typed
open import Definition.Typed.Properties
import Definition.Typed.Weakening as Wk
open import Definition.LogicalRelation
open import Definition.LogicalRelation.ShapeView
open import Definition.LogicalRelation.Irrelevance
open import Definition.LogicalRelation.Properties.Reflexivity
open import Definition.LogicalRelation.Properties.Escape
open import Definition.LogicalRelation.Properties.Symmetry

open import Tools.Nat
open import Tools.Product
import Tools.PropositionalEquality as PE

private
  variable
    m : Nat
    Γ : Con Term m

-- Neutral reflexive types are reducible.
neu : ∀ {l A} (neA : Neutral A)
    → Γ ⊢ A
    → Γ ⊢ A ~ A ∷ U
    → Γ ⊩⟨ l ⟩ A
neu neA A A~A = ne′ _ (idRed:*: A) neA A~A

  -- Helper function for reducible neutral equality of a specific type of derivation.
neuEq′ : ∀ {l A B} ([A] : Γ ⊩⟨ l ⟩ne A)
         (neA : Neutral A)
         (neB : Neutral B)
       → Γ ⊢ A → Γ ⊢ B
       → Γ ⊢ A ~ B ∷ U
       → Γ ⊩⟨ l ⟩ A ≡ B / ne-intr [A]
neuEq′ (noemb (ne K [ ⊢A , ⊢B , D ] neK K≡K)) neA neB A B A~B =
  let A≡K = whnfRed* D (ne neA)
  in  ne₌ _ (idRed:*: B) neB (PE.subst (λ x → _ ⊢ x ~ _ ∷ _) A≡K A~B)
neuEq′ (emb 0<1 x) neB A:≡:B = neuEq′ x neB A:≡:B

-- Neutrally equal types are of reducible equality.
neuEq : ∀ {l A B} ([A] : Γ ⊩⟨ l ⟩ A)
        (neA : Neutral A)
        (neB : Neutral B)
      → Γ ⊢ A → Γ ⊢ B
      → Γ ⊢ A ~ B ∷ U
      → Γ ⊩⟨ l ⟩ A ≡ B / [A]
neuEq [A] neA neB A B A~B =
  irrelevanceEq (ne-intr (ne-elim neA [A]))
                [A]
                (neuEq′ (ne-elim neA [A]) neA neB A B A~B)

mutual
  -- Neutral reflexive terms are reducible.
  neuTerm : ∀ {l A n} ([A] : Γ ⊩⟨ l ⟩ A) (neN : Neutral n)
          → Γ ⊢ n ∷ A
          → Γ ⊢ n ~ n ∷ A
          → Γ ⊩⟨ l ⟩ n ∷ A / [A]
  neuTerm (Uᵣ′ .⁰ 0<1 ⊢Γ) neN n n~n =
    Uₜ _ (idRedTerm:*: n) (ne neN) (~-to-≅ₜ n~n) (neu neN (univ n) n~n)
  neuTerm (ℕᵣ [ ⊢A , ⊢B , D ]) neN n n~n =
    let A≡ℕ  = subset* D
        n~n′ = ~-conv n~n A≡ℕ
        n≡n  = ~-to-≅ₜ n~n′
    in  ℕₜ _ (idRedTerm:*: (conv n A≡ℕ)) n≡n (ne (neNfₜ neN (conv n A≡ℕ) n~n′))
  neuTerm (Emptyᵣ [ ⊢A , ⊢B , D ]) neN n n~n =
    let A≡Empty  = subset* D
        n~n′ = ~-conv n~n A≡Empty
        n≡n  = ~-to-≅ₜ n~n′
    in  Emptyₜ _ (idRedTerm:*: (conv n A≡Empty)) n≡n (ne (neNfₜ neN (conv n A≡Empty) n~n′))
  neuTerm (Unitᵣ [ ⊢A , ⊢B , D ]) neN n n~n =
    let A≡Unit  = subset* D
        n~n′ = ~-conv n~n A≡Unit
    in  Unitₜ _ (idRedTerm:*: (conv n A≡Unit))
              (~-to-≅ₜ (~-conv n~n A≡Unit))
              (ne (neNfₜ neN (conv n A≡Unit) (~-conv n~n A≡Unit)))
  neuTerm (ne′ K [ ⊢A , ⊢B , D ] neK K≡K) neN n n~n =
    let A≡K = subset* D
    in  neₜ _ (idRedTerm:*: (conv n A≡K)) (neNfₜ neN (conv n A≡K)
            (~-conv n~n A≡K))
  neuTerm (Πᵣ′ F G D ⊢F ⊢G A≡A [F] [G] G-ext) neN n n~n =
    let A≡ΠFG = subset* (red D)
    in  Πₜ _ (idRedTerm:*: (conv n A≡ΠFG)) (ne neN) (~-to-≅ₜ (~-conv n~n A≡ΠFG))
           (λ {_} {ρ} [ρ] ⊢Δ [a] [b] [a≡b] →
              let A≡ΠFG = subset* (red D)
                  ρA≡ρΠFG = Wk.wkEq [ρ] ⊢Δ (subset* (red D))
                  G[a]≡G[b] = escapeEq ([G] [ρ] ⊢Δ [b])
                                          (symEq ([G] [ρ] ⊢Δ [a]) ([G] [ρ] ⊢Δ [b])
                                                 (G-ext [ρ] ⊢Δ [a] [b] [a≡b]))
                  a = escapeTerm ([F] [ρ] ⊢Δ) [a]
                  b = escapeTerm ([F] [ρ] ⊢Δ) [b]
                  a≡b = escapeTermEq ([F] [ρ] ⊢Δ) [a≡b]
                  ρn = conv (Wk.wkTerm [ρ] ⊢Δ n) ρA≡ρΠFG
                  neN∘a = ∘ₙ (wkNeutral ρ neN)
                  neN∘b = ∘ₙ (wkNeutral ρ neN)
              in  neuEqTerm ([G] [ρ] ⊢Δ [a]) neN∘a neN∘b
                            (ρn ∘ⱼ a)
                            (conv (ρn ∘ⱼ b) (≅-eq G[a]≡G[b]))
                            (~-app (~-wk [ρ] ⊢Δ (~-conv n~n A≡ΠFG)) a≡b))
           (λ {_} {ρ} [ρ] ⊢Δ [a] →
              let ρA≡ρΠFG = Wk.wkEq [ρ] ⊢Δ (subset* (red D))
                  a = escapeTerm ([F] [ρ] ⊢Δ) [a]
                  a≡a = escapeTermEq ([F] [ρ] ⊢Δ) (reflEqTerm ([F] [ρ] ⊢Δ) [a])
              in  neuTerm ([G] [ρ] ⊢Δ [a]) (∘ₙ (wkNeutral ρ neN))
                          (conv (Wk.wkTerm [ρ] ⊢Δ n) ρA≡ρΠFG ∘ⱼ a)
                          (~-app (~-wk [ρ] ⊢Δ (~-conv n~n A≡ΠFG)) a≡a))
  neuTerm (Σᵣ′ F G D ⊢F ⊢G A≡A [F] [G] G-ext) neN ⊢n n~n =
    let A≡ΣFG = subset* (red D)
        ⊢Γ = wf ⊢F
        ⊢n = conv ⊢n A≡ΣFG
        n~n = ~-conv n~n A≡ΣFG

        [F] = [F] Wk.id ⊢Γ
        [fst] = neuTerm [F] (fstₙ neN)
                        (PE.subst
                          (λ x → _ ⊢ fst _ ∷ x)
                          (PE.sym (wk-id F))
                          (fstⱼ ⊢F ⊢G ⊢n))
                        (PE.subst
                          (λ x → _ ⊢ _ ~ _ ∷ x)
                          (PE.sym (wk-id F))
                          (~-fst ⊢F ⊢G n~n))
        [Gfst] = [G] Wk.id ⊢Γ [fst]
        [snd] = neuTerm [Gfst] (sndₙ neN)
                        (PE.subst
                          (λ x → _ ⊢ snd _ ∷ x)
                          (PE.cong (λ x → x [ fst _ ]) (PE.sym (wk-lift-id G)))
                          (sndⱼ ⊢F ⊢G ⊢n))
                        (PE.subst
                          (λ x → _ ⊢ _ ~ _ ∷ x)
                          (PE.cong (λ x → x [ fst _ ]) (PE.sym (wk-lift-id G)))
                          (~-snd ⊢F ⊢G n~n))
    in  Σₜ _ (idRedTerm:*: ⊢n) (ne neN) (~-to-≅ₜ n~n)
           [fst]
           [snd]
  neuTerm (∪ᵣ′ F G D ⊢F ⊢G A≡A [F] [G]) neN ⊢n n~n =
    ∪₃ₜ _ (idRedTerm:*: (conv ⊢n (subset* (red D))))
        (~-to-≅ₜ (~-conv n~n (subset* (red D))))
        (neNfₜ neN (conv ⊢n (subset* (red D))) (~-conv n~n (subset* (red D))))
  neuTerm (∥ᵣ′ F D ⊢F A≡A [F]) neN ⊢n n~n =
    ∥₂ₜ _ (idRedTerm:*: (conv ⊢n (subset* (red D))))
        (~-to-≅ₜ (~-conv n~n (subset* (red D))))
        (neNfₜ neN (conv ⊢n (subset* (red D))) (~-conv n~n (subset* (red D))))
  neuTerm (emb 0<1 x) neN n = neuTerm x neN n

  -- Neutrally equal terms are of reducible equality.
  neuEqTerm : ∀ {l A n n′} ([A] : Γ ⊩⟨ l ⟩ A)
              (neN : Neutral n) (neN′ : Neutral n′)
            → Γ ⊢ n  ∷ A
            → Γ ⊢ n′ ∷ A
            → Γ ⊢ n ~ n′ ∷ A
            → Γ ⊩⟨ l ⟩ n ≡ n′ ∷ A / [A]
  neuEqTerm (Uᵣ′ .⁰ 0<1 ⊢Γ) neN neN′ n n′ n~n′ =
    let [n]  = neu neN  (univ n) (~-trans n~n′ (~-sym n~n′))
        [n′] = neu neN′ (univ n′) (~-trans (~-sym n~n′) n~n′)
    in  Uₜ₌ _ _ (idRedTerm:*: n) (idRedTerm:*: n′) (ne neN) (ne neN′)
            (~-to-≅ₜ n~n′) [n] [n′] (neuEq [n] neN neN′ (univ n) (univ n′) n~n′)
  neuEqTerm (ℕᵣ [ ⊢A , ⊢B , D ]) neN neN′ n n′ n~n′ =
    let A≡ℕ = subset* D
        n~n′₁ = ~-conv n~n′ A≡ℕ
        n≡n′ = ~-to-≅ₜ n~n′₁
    in  ℕₜ₌ _ _ (idRedTerm:*: (conv n A≡ℕ)) (idRedTerm:*: (conv n′ A≡ℕ))
            n≡n′ (ne (neNfₜ₌ neN neN′ n~n′₁))
  neuEqTerm (Emptyᵣ [ ⊢A , ⊢B , D ]) neN neN′ n n′ n~n′ =
    let A≡Empty = subset* D
        n~n′₁ = ~-conv n~n′ A≡Empty
        n≡n′ = ~-to-≅ₜ n~n′₁
    in  Emptyₜ₌ _ _ (idRedTerm:*: (conv n A≡Empty)) (idRedTerm:*: (conv n′ A≡Empty))
            n≡n′ (ne (neNfₜ₌ neN neN′ n~n′₁))
  neuEqTerm (Unitᵣ [ ⊢A , ⊢B , D ]) neN neN′ n n′ n~n′ =
    let A≡Unit = subset* D
    in  Unitₜ₌ _ _ (idRedTerm:*: (conv n A≡Unit)) (idRedTerm:*: (conv n′ A≡Unit))
               (~-to-≅ₜ (~-conv n~n′ A≡Unit))
               (ne (neNfₜ neN (conv n A≡Unit) (~-conv (~-trans n~n′ (~-sym n~n′)) A≡Unit)) ,
                ne (neNfₜ neN′ (conv n′ A≡Unit) (~-conv (~-trans (~-sym n~n′) n~n′) A≡Unit)))
 --(ne (neNfₜ₌ neN neN′ (~-conv n~n′ A≡Unit)))
  neuEqTerm (ne (ne K [ ⊢A , ⊢B , D ] neK K≡K)) neN neN′ n n′ n~n′ =
    let A≡K = subset* D
    in  neₜ₌ _ _ (idRedTerm:*: (conv n A≡K)) (idRedTerm:*: (conv n′ A≡K))
             (neNfₜ₌ neN neN′ (~-conv n~n′ A≡K))
  neuEqTerm (Πᵣ′ F G [ ⊢A , ⊢B , D ] ⊢F ⊢G A≡A [F] [G] G-ext) neN neN′ n n′ n~n′ =
    let [ΠFG] = Πᵣ′ F G [ ⊢A , ⊢B , D ] ⊢F ⊢G A≡A [F] [G] G-ext
        A≡ΠFG = subset* D
        n~n′₁ = ~-conv n~n′ A≡ΠFG
        n≡n′ = ~-to-≅ₜ n~n′₁
        n~n = ~-trans n~n′ (~-sym n~n′)
        n′~n′ = ~-trans (~-sym n~n′) n~n′
    in  Πₜ₌ _ _ (idRedTerm:*: (conv n A≡ΠFG)) (idRedTerm:*: (conv n′ A≡ΠFG))
            (ne neN) (ne neN′) n≡n′
            (neuTerm [ΠFG] neN n n~n) (neuTerm [ΠFG] neN′ n′ n′~n′)
            (λ {_} {ρ} [ρ] ⊢Δ [a] →
               let ρA≡ρΠFG = Wk.wkEq [ρ] ⊢Δ A≡ΠFG
                   ρn = Wk.wkTerm [ρ] ⊢Δ n
                   ρn′ = Wk.wkTerm [ρ] ⊢Δ n′
                   a = escapeTerm ([F] [ρ] ⊢Δ) [a]
                   a≡a = escapeTermEq ([F] [ρ] ⊢Δ)
                                          (reflEqTerm ([F] [ρ] ⊢Δ) [a])
                   neN∙a   = ∘ₙ (wkNeutral ρ neN)
                   neN′∙a′ = ∘ₙ (wkNeutral ρ neN′)
               in  neuEqTerm ([G] [ρ] ⊢Δ [a]) neN∙a neN′∙a′
                             (conv ρn  ρA≡ρΠFG ∘ⱼ a)
                             (conv ρn′ ρA≡ρΠFG ∘ⱼ a)
                             (~-app (~-wk [ρ] ⊢Δ n~n′₁) a≡a))
  neuEqTerm (Σᵣ′ F G [ ⊢A , ⊢B , D ] ⊢F ⊢G A≡A [F] [G] G-ext) neN neN′ ⊢n ⊢n′ n~n′ =
    let [ΣFG] = Σᵣ′ F G [ ⊢A , ⊢B , D ] ⊢F ⊢G A≡A [F] [G] G-ext
        A≡ΣFG = subset* D
        n~n = ~-trans n~n′ (~-sym n~n′)
        n′~n′ = ~-trans (~-sym n~n′) n~n′

        ⊢Γ = wf ⊢F
        ⊢nΣ = conv ⊢n A≡ΣFG
        ⊢n′Σ = conv ⊢n′ A≡ΣFG
        n~n′Σ = ~-conv n~n′ A≡ΣFG
        n~nΣ = ~-conv n~n A≡ΣFG
        n′~n′Σ = ~-conv n′~n′ A≡ΣFG
        [F] = [F] Wk.id ⊢Γ
        ⊢fstnΣ = (PE.subst
                (λ x → _ ⊢ fst _ ∷ x)
                (PE.sym (wk-id F))
                (fstⱼ ⊢F ⊢G ⊢nΣ))
        ⊢fstn′Σ = (PE.subst
                    (λ x → _ ⊢ fst _ ∷ x)
                    (PE.sym (wk-id F))
                    (fstⱼ ⊢F ⊢G ⊢n′Σ))
        [fstn] = neuTerm [F] (fstₙ neN)
                         ⊢fstnΣ
                         (PE.subst
                           (λ x → _ ⊢ _ ~ _ ∷ x)
                           (PE.sym (wk-id F))
                           (~-fst ⊢F ⊢G n~nΣ))
        [fstn′] = neuTerm [F] (fstₙ neN′)
                          ⊢fstn′Σ
                          (PE.subst
                            (λ x → _ ⊢ _ ~ _ ∷ x)
                            (PE.sym (wk-id F))
                            (~-fst ⊢F ⊢G n′~n′Σ))
        [fstn≡fstn′] = neuEqTerm [F] (fstₙ neN) (fstₙ neN′)
                         ⊢fstnΣ
                         ⊢fstn′Σ
                         (PE.subst
                           (λ x → _ ⊢ _ ~ _ ∷ x)
                           (PE.sym (wk-id F))
                           (~-fst ⊢F ⊢G n~n′Σ))
        [Gfstn] = [G] Wk.id ⊢Γ [fstn]
        [Gfstn′] = PE.subst (λ x → _ ⊩⟨ _ ⟩ x [ fst _ ]) (wk-lift-id G) ([G] Wk.id ⊢Γ [fstn′])
        [fstn′≡fstn] = symEqTerm [F] [fstn≡fstn′]
        [Gfstn′≡Gfstn] = irrelevanceEq″
                           (PE.cong (λ x → x [ fst _ ]) (wk-lift-id G))
                           (PE.cong (λ x → x [ fst _ ]) (wk-lift-id G))
                           ([G] Wk.id ⊢Γ [fstn′]) [Gfstn′]
                           (G-ext Wk.id ⊢Γ [fstn′] [fstn] [fstn′≡fstn])
        Gfstn′≡Gfstn = ≅-eq (escapeEq [Gfstn′] [Gfstn′≡Gfstn])
        [sndn≡sndn′] = neuEqTerm [Gfstn] (sndₙ neN) (sndₙ neN′)
                          (PE.subst
                            (λ x → _ ⊢ snd _ ∷ x)
                            (PE.cong (λ x → x [ fst _ ]) (PE.sym (wk-lift-id G)))
                            (sndⱼ ⊢F ⊢G ⊢nΣ))
                          (PE.subst
                            (λ x → _ ⊢ snd _ ∷ x)
                            (PE.cong (λ x → x [ fst _ ]) (PE.sym (wk-lift-id G)))
                            (conv (sndⱼ ⊢F ⊢G ⊢n′Σ) Gfstn′≡Gfstn))
                          (PE.subst
                            (λ x → _ ⊢ _ ~ _ ∷ x)
                            (PE.cong (λ x → x [ fst _ ]) (PE.sym (wk-lift-id G)))
                            (~-snd ⊢F ⊢G n~n′Σ))
    in  Σₜ₌ _ _ (idRedTerm:*: ⊢nΣ) (idRedTerm:*: ⊢n′Σ)
            (ne neN) (ne neN′) (~-to-≅ₜ n~n′Σ)
            (neuTerm [ΣFG] neN ⊢n n~n) (neuTerm [ΣFG] neN′ ⊢n′ n′~n′)
            [fstn] [fstn′] [fstn≡fstn′] [sndn≡sndn′]
  neuEqTerm (∪ᵣ′ F G [ ⊢A , ⊢B , D ] ⊢F ⊢G A≡A [F] [G]) neN neN′ ⊢n ⊢n′ n~n′ =
    ∪₃ₜ₌ _ _
         (idRedTerm:*: (conv ⊢n (subset* D)))
         (idRedTerm:*: (conv ⊢n′ (subset* D)))
         (≅-conv (~-to-≅ₜ n~n′) (subset* D))
         (neuTerm (∪ᵣ′ F G [ ⊢A , ⊢B , D ] ⊢F ⊢G A≡A [F] [G]) neN ⊢n (~-trans n~n′ (~-sym n~n′)))
         (neuTerm (∪ᵣ′ F G [ ⊢A , ⊢B , D ] ⊢F ⊢G A≡A [F] [G]) neN′ ⊢n′ (~-trans (~-sym n~n′) n~n′))
         (neNfₜ₌ neN neN′ (~-conv n~n′ (subset* D)))
  neuEqTerm (∥ᵣ′ F [ ⊢A , ⊢B , D ] ⊢F A≡A [F]) neN neN′ ⊢n ⊢n′ n~n′ =
    ∥₂ₜ₌ _ _
         (idRedTerm:*: (conv ⊢n (subset* D)))
         (idRedTerm:*: (conv ⊢n′ (subset* D)))
         (≅-conv (~-to-≅ₜ n~n′) (subset* D))
         (neuTerm (∥ᵣ′ F [ ⊢A , ⊢B , D ] ⊢F A≡A [F]) neN ⊢n (~-trans n~n′ (~-sym n~n′)))
         (neuTerm (∥ᵣ′ F [ ⊢A , ⊢B , D ] ⊢F A≡A [F]) neN′ ⊢n′ (~-trans (~-sym n~n′) n~n′))
         (neNfₜ₌ neN neN′ (~-conv n~n′ (subset* D)))
  neuEqTerm (emb 0<1 x) neN neN′ n:≡:n′ = neuEqTerm x neN neN′ n:≡:n′
